Simplify check for valkid indexing.

src/dafny/smart/Trees2.dfy
@@ -15,7 +15,7 @@
 include "Helpers.dfy"
 
 /**
- *  Provide tree decorated with value.
+ *  Provide tree decorated with value and indexed trees.
  */
 module Trees {
 
@@ -23,10 +23,9 @@ module Trees {
 
     newtype{:nativeType "int"} bit = i:int | 0 <= i < 2
 
-    /** Binary trees.
+    /** 
+     *  Binary trees.
      *
-     *  Values are in a domain `T`.
-     *  
      *  @tparam T   The type of values attached to the nodes.
      *  @param  v   The value associated with a node.
      */
@@ -34,13 +33,12 @@ module Trees {
             Leaf(v: T)
         |   Node(v: T, left: Tree, right: Tree)
 
-    /** Binary trees with an index.
-     *
-     *  Values are in a domain `T`.
+    /** 
+     *  Binary trees with node identifier.
      *  
      *  @tparam T   The type of values attached to the nodes.
      *  @param  v   The value associated with a node.
-     8  @param  id  A sequence that corresponds to the node id.
+     *  @param  id  A sequence that corresponds to the node id.
      */
     datatype ITree<T> = 
             ILeaf(v: T, ghost id: seq<bit>)
@@ -48,23 +46,48 @@ module Trees {
 
     /**
      *  Height of a tree.
+     *
+     *  @param  root    The root of the tree.
+     *  @returns        The height of the tree.
      */
     function height(root : ITree) : nat 
         ensures height(root) >= 1
         decreases root
     {
         match root 
-            //  a leaf has height 1
             case ILeaf(_, _) => 1
-            //  A node has height 1 + max height of children
             case INode(_, lc, rc, _) => 1 + max(height(lc), height(rc))
     }
 
     /**
+     *  Whether a tree is properly indexed (lexicographic order)
+     *  from an initial value `p`.   
+     *  
+     *  @param  r   The root of the tree.
+     *  @param  p   The prefix used for the id. 
+     */
+    predicate isValidIndex(r: ITree, p : seq<bit>) 
+        decreases r
+    {
+       match r 
+            case ILeaf(_, id) => id == p
+
+            case INode(_, lc, rc, id) =>
+                id == p && isValidIndex(lc, p + [0]) && isValidIndex(rc, p + [1]) 
+    }
+
+    /**
      *  Make an indexed tree from a tree.
+     *
+     *  @param  r   The root of the tree.
+     *  @param  p   The prefix to use in indexing.
+     *  @returns    A indexed tree where each node has an index as
+     *              a sequence of 0 (left) and 1 (right). The id of 
+     *              corresponds to the path from the root. 
      */
     function indexFrom<T>(r : Tree<T>, p : seq<bit>) : ITree<T> 
-        // ensures forall n :: n in nodesIn(indexFrom(r, p)) ==> |n.id| >= |p| 
+        ensures {:induction r} forall n :: n in nodesIn(indexFrom(r, p)) ==> |n.id| >= |p| 
+        ensures isValidIndex(indexFrom(r, p), p)
         decreases r
     {
         match r 
@@ -73,27 +96,59 @@ module Trees {
                 INode(v, indexFrom(lc, p + [0]), indexFrom(rc, p + [1]), p)
     }
 
-    lemma {:induction r} indexFromMonotonic(r : Tree, t : ITree, p : seq<bit>, n : nat)
-        requires t == indexFrom(r, p)
-        requires 0 <= n < |nodesIn(t)|
-        ensures p <= nodesIn(t)[n]. id 
-        decreases r 
-    {
-        match r 
-            case Leaf(_) =>
+    
 
-            case Node(_, lc, rc) => 
-                assert(t.INode?);
-                match t 
-                    case INode(_, tlc, trc, id) =>
-                        assert(nodesIn(t) == [t] + nodesIn(tlc) + nodesIn(trc));
-                        if ( n == 0 ) {
-                            //  Thanks Dafny
-                        }  else if ( 1 <= n <= |nodesIn(tlc)|) {
-                            indexFromMonotonic(lc, tlc, p + [0], n - 1);
-                        } else {
-                            indexFromMonotonic(rc, trc, p + [1], n - 1 - |nodesIn(tlc)|);
-                        }
+    // lemma foo32(r : ITree, p : seq<bit>) 
+    //     requires isValidIndex(r, p) 
+    //     ensures p <= r.id 
+    // {}
+
+    /**
+     *  Index from an intial value 
+     */
+    // lemma {:induction r} indexFromMonotonic(r : Tree, t : ITree, p : seq<bit>, n : nat)
+    //     requires t == indexFrom(r, p)
+    //     requires 0 <= n < |nodesIn(t)|
+    //     ensures p <= nodesIn(t)[n]. id 
+    //     decreases r 
+    // {
+    //     match r 
+    //         case Leaf(_) =>
+
+    //         case Node(_, lc, rc) => 
+    //             assert(t.INode?);
+    //             match t 
+    //                 case INode(_, tlc, trc, id) =>
+    //                     assert(nodesIn(t) == [t] + nodesIn(tlc) + nodesIn(trc));
+    //                     if ( n == 0 ) {
+    //                         //  Thanks Dafny
+    //                     }  else if ( 1 <= n <= |nodesIn(tlc)|) {
+    //                         indexFromMonotonic(lc, tlc, p + [0], n - 1);
+    //                     } else {
+    //                         indexFromMonotonic(rc, trc, p + [1], n - 1 - |nodesIn(tlc)|);
+    //                     }
+    // }
+
+    /**
+     *  Index of each node of a indexed that is valid is >= `p`.
+     */
+    lemma {:induction t} indexFromMonotonic2(t : ITree, p : seq<bit>, n : nat)
+        requires isValidIndex(t, p) 
+        requires 0 <= n < |nodesIn(t)|
+        ensures p <= nodesIn(t)[n].id 
+        decreases t 
+    {
+        match t 
+            case ILeaf(_, _) =>
+
+            case INode(_, lc, rc, _) => 
+                if ( n == 0 ) {
+                    //  Thanks Dafny
+                }  else if ( 1 <= n <= |nodesIn(lc)|) {
+                    indexFromMonotonic2(lc, p + [0], n - 1);
+                } else {
+                    indexFromMonotonic2(rc, p + [1], n - 1 - |nodesIn(lc)|);
+                }
     }
 
     /**
@@ -199,6 +254,86 @@ module Trees {
                 }
     }
 
+    lemma {:induction r} uniqueNodeId2(r: ITree, k1 : nat, k2 : nat, p : seq<bit>) 
+        requires isValidIndex(r, p) 
+        requires 0 <= k1 < k2 < |nodesIn(r)|
+        ensures nodesIn(r)[k1].id != nodesIn(r)[k2].id
+        decreases r
+    {
+        match r 
+            case ILeaf(v, id) => // Vacuously true. Thanks Dafny
+
+            case INode(v, lc, rc, id) =>
+
+                // assert( nodesIn(r) == [r] + nodesIn(lc) + nodesIn(rc));
+                if ( k1 == 0 ) {
+                    //  ids in lc and rc have length r.id + 1
+                    assert(p < nodesIn(r)[k2].id);
+                } else if 1 <= k1 < k2 <= |nodesIn(lc)| {
+                    //  both indices are nodes in lc
+                    assert(0 <= k1 - 1 < k2 - 1 < |nodesIn(lc)|);
+                    // assert(t.Node?);
+                    // match t 
+                    //     case Node(_, tlc, _) => 
+                    //         assert(lc == indexFrom(tlc, p + [0]));
+                    uniqueNodeId2(lc, k1 - 1, k2 - 1, p + [0]);
+                } else if 1 + |nodesIn(lc)| <= k1 < k2 < |nodesIn(r)| {
+                    //  both indices are nodes in rc
+                    var i1 := k1 - 1 - |nodesIn(lc)|;
+                    var i2 := k2 - 1 - |nodesIn(lc)|;
+                    assert(0 <= i1 < i2 < |nodesIn(rc)|);
+                    // assert(t.Node?);
+                    // match t 
+                    //     case Node(_, _, trc) => 
+                    //         assert(rc == indexFrom(trc, p + [1]));
+                    uniqueNodeId2(rc, i1, i2, p + [1]);
+                } else {
+                    //  k1 indexed a node in lc and k2 a node in rc
+                    assert ( 1 <= k1 < 1 + |nodesIn(lc)| <= k2 < |nodesIn(r)| );
+                    // assert(t.Node?);
+                    // match t 
+                        // case Node(_, tlc, trc) =>
+                        //     assert(lc == indexFrom(tlc, p + [0]));
+                        var i1 := k1 - 1;
+                        indexFromMonotonic2(lc, p + [0], i1);
+
+                        // assert(rc == indexFrom(trc, p + [1]));
+                        var i2 := k2 - 1 - |nodesIn(lc)|;
+                        indexFromMonotonic2(rc, p + [1], i2);
+
+                        assert(p + [0] <= nodesIn(r)[k1].id );
+                        assert(p + [1] <= nodesIn(r)[k2].id );
+
+                        //  Prove post condition by contradiction
+                        calc ==> {
+                            nodesIn(r)[k1].id == nodesIn(r)[k2].id ;
+                            ==>
+                            nodesIn(r)[k1].id[..|p| + 1] == nodesIn(r)[k2].id[..|p| + 1] ;
+                            ==> calc == {
+                                    p + [0] ;
+                                    ==
+                                    (p + [0])[..|p| + 1];
+                                    == 
+                                    nodesIn(r)[k1].id[..|p| + 1];
+                            }
+                            p + [0] == nodesIn(r)[k2].id[..|p| + 1] ;
+                            ==> calc == {
+                                    p + [1] ;
+                                    ==
+                                    (p + [1])[..|p| + 1];
+                                    == 
+                                    nodesIn(r)[k2].id[..|p| + 1];
+                            }
+                            p + [0] == p + [1];
+                            ==>
+                            (p + [0])[|p|] == (p + [1])[|p|];
+                            ==>
+                            //  contradiction
+                            0 == 1;
+                        }
+                }
+    }
+    
     /**
      *  The node at the end of a path.
      *
